PhysLean/Particles/SuperSymmetry/SU5/Charges/PhenoClosed.lean
@@ -1,0 +1,228 @@
+/-
+Copyright (c) 2025 Joseph Tooby-Smith. All rights reserved.
+Released under Apache 2.0 license as described in the file LICENSE.
+Authors: Joseph Tooby-Smith
+-/
+import PhysLean.Particles.SuperSymmetry.SU5.Charges.PhenoConstrained
+import PhysLean.Particles.SuperSymmetry.SU5.Charges.Yukawa
+import PhysLean.Particles.SuperSymmetry.SU5.Charges.Completions
+import PhysLean.Particles.SuperSymmetry.SU5.Charges.MinimallyAllowsTerm.OfFinset
+import PhysLean.Particles.SuperSymmetry.SU5.Charges.MinimalSuperSet
+/-!
+
+# Phenomenologically closed sets of charges
+
+In this module we define a number of propositions related to the phenomenological closure of
+sets of charges.
+
+One of the key results within this module is the lemma
+`completeness_of_isPhenoClosedQ5_isPhenoClosedQ10`, which gives a quick way to
+check whether a set of charges contains precisely those charges which
+- allow the top Yukawa term,
+- are not phenomenologically constrained,
+- do not generate dangerous couplings with one singlet insertion,
+- and are complete,
+given allowed values of `5`d and `10`d charges `S5` and `S10`.
+This result can be used for specific sets of charges `S5` and `S10`, along with
+some results proved by `decide`.
+
+-/
+namespace SuperSymmetry
+
+namespace SU5
+
+namespace Charges
+
+variable {𝓩 : Type} [DecidableEq 𝓩] [AddCommGroup 𝓩]
+
+/-!
+
+## IsPhenoClosedQ5
+
+-/
+
+/-- The proposition that for multiset set of charges `charges`,
+  adding individual elements of `S5` to the `Q5` charges of elements of `charges` again
+  leads to an element in `charges` or a charge which is phenomenologically constrained,
+  or regenerates dangerous couplings with one singlet insertion. -/
+def IsPhenoClosedQ5 (S5 : Finset 𝓩) (charges : Multiset (Charges 𝓩)) : Prop :=
+  ∀ q5 ∈ S5, ∀ x ∈ charges,
+    let y : Charges 𝓩 := (x.1, x.2.1, insert q5 x.2.2.1, x.2.2.2)
+    IsPhenoConstrained y ∨ y ∈ charges ∨ YukawaGeneratesDangerousAtLevel y 1
+
+lemma isPhenClosedQ5_of_isPhenoConstrainedQ5 {S5 : Finset 𝓩} {charges : Multiset (Charges 𝓩)}
+    (h : ∀ q5 ∈ S5, ∀ x ∈ charges,
+      let y : Charges 𝓩 := (x.1, x.2.1, insert q5 x.2.2.1, x.2.2.2)
+      IsPhenoConstrainedQ5 x q5 ∨ y ∈ charges ∨ YukawaGeneratesDangerousAtLevel y 1) :
+    IsPhenoClosedQ5 S5 charges := by
+  intro q5 hq5 x hx
+  have h' := h q5 hq5 x hx
+  rcases h' with h'| h' | h'
+  · left
+    rw [isPhenoConstrained_insertQ5_iff_isPhenoConstrainedQ5]
+    left
+    exact h'
+  · simp_all
+  · simp_all
+
+/-!
+
+## IsPhenoClosedQ10
+
+-/
+
+/-- The proposition that for multiset set of charges `charges`,
+  adding individual elements of `S10` to the `Q10` charges of elements of `charges` again
+  leads to an element in `charges` or a charge which is phenomenologically constrained,
+  or regenerates dangerous couplings with one singlet insertion. -/
+def IsPhenoClosedQ10 (S10 : Finset 𝓩) (charges : Multiset (Charges 𝓩)) : Prop :=
+  ∀ q10 ∈ S10, ∀ x ∈ charges,
+    let y : Charges 𝓩 := (x.1, x.2.1, x.2.2.1, insert q10 x.2.2.2)
+    IsPhenoConstrained y ∨ y ∈ charges ∨ YukawaGeneratesDangerousAtLevel y 1
+
+lemma isPhenClosedQ10_of_isPhenoConstrainedQ10 {S10 : Finset 𝓩} {charges : Multiset (Charges 𝓩)}
+    (h : ∀ q10 ∈ S10, ∀ x ∈ charges,
+      let y : Charges 𝓩 := (x.1, x.2.1, x.2.2.1, insert q10 x.2.2.2)
+      IsPhenoConstrainedQ10 x q10 ∨ y ∈ charges ∨ YukawaGeneratesDangerousAtLevel y 1) :
+    IsPhenoClosedQ10 S10 charges := by
+  intro q10 hq10 x hx
+  have h' := h q10 hq10 x hx
+  rcases h' with h'| h' | h'
+  · left
+    rw [isPhenoConstrained_insertQ10_iff_isPhenoConstrainedQ10]
+    left
+    exact h'
+  · simp_all
+  · simp_all
+
+open PotentialTerm
+
+/-- The proposition that for multiset set of charges `charges` contains all
+  viable completions of charges which allow the top Yukawa, given allowed values
+  of `5`d and `10`d charges `S5` and `S10`. -/
+def ContainsPhenoCompletionsOfMinimallyAllows (S5 S10 : Finset 𝓩) (charges : Multiset (Charges 𝓩)) :
+    Prop := ∀ x ∈ (minimallyAllowsTermsOfFinset S5 S10 topYukawa),
+      ¬ x.IsPhenoConstrained → ∀ y ∈ completions S5 S10 x, ¬ y.IsPhenoConstrained
+      ∧ ¬ y.YukawaGeneratesDangerousAtLevel 1 → y ∈ charges
+
+instance [DecidableEq 𝓩] {S5 S10 : Finset 𝓩} {charges : Multiset (Charges 𝓩)} :
+    Decidable (ContainsPhenoCompletionsOfMinimallyAllows S5 S10 charges) :=
+  Multiset.decidableForallMultiset
+
+lemma containsPhenoCompletionsOfMinimallyAllows_of_subset {S5 S10 : Finset 𝓩}
+    {charges charges' : Multiset (Charges 𝓩)}
+    (h' : ContainsPhenoCompletionsOfMinimallyAllows S5 S10 charges)
+    (h : ∀ x ∈ charges, x ∈ charges') :
+    ContainsPhenoCompletionsOfMinimallyAllows S5 S10 charges' := by
+  intro x hx hnot y h3 h4
+  apply h
+  exact h' x hx hnot y h3 h4
+
+/-!
+
+## Completeness of isPhenoClosedQ5 and isPhenoClosedQ10
+
+-/
+
+/-!
+The multiset of charges `charges` contains precisely those charges (given a finite set
+of allowed charges) which
+- allow the top Yukawa term,
+- are not phenomenologically constrained,
+- do not generate dangerous couplings with one singlet insertion,
+- and are complete,
+if the following conditions hold:
+- every element of `charges` allows the top Yukawa term,
+- every element of `charges` is not phenomenologically constrained,
+- every element of `charges` does not generate dangerous couplings with one singlet insertion,
+- every element of `charges` is complete,
+- `charges` is `IsPhenoClosedQ5` with respect to `S5`,
+- `charges` is `IsPhenoClosedQ10` with respect to `S10`
+- and satisfies `ContainsPhenoCompletionsOfMinimallyAllows S5 S10 charges`.
+The importance of this lemma is that it is only regarding properties of finite-set `charges`
+not of the whole space of possible charges.
+-/
+lemma completeness_of_isPhenoClosedQ5_isPhenoClosedQ10
+    {S5 S10 : Finset 𝓩} {charges : Multiset (Charges 𝓩)}
+    (charges_topYukawa : ∀ x ∈ charges, x.AllowsTerm .topYukawa)
+    (charges_not_isPhenoConstrained : ∀ x ∈ charges, ¬ x.IsPhenoConstrained)
+    (charges_yukawa : ∀ x ∈ charges, ¬ x.YukawaGeneratesDangerousAtLevel 1)
+    (charges_complete : ∀ x ∈ charges, x.IsComplete)
+    (charges_isPhenoClosedQ5 : IsPhenoClosedQ5 S5 charges)
+    (charges_isPhenoClosedQ10 : IsPhenoClosedQ10 S10 charges)
+    (charges_exist : ContainsPhenoCompletionsOfMinimallyAllows S5 S10 charges)
+    {x : Charges 𝓩} (hsub : x ∈ ofFinset S5 S10) :
+    x ∈ charges ↔ AllowsTerm x .topYukawa ∧
+    ¬ IsPhenoConstrained x ∧ ¬ YukawaGeneratesDangerousAtLevel x 1 ∧ IsComplete x := by
+  constructor
+  · /- Showing that if `x ∈ Charges` it satifies the conditions. -/
+    intro h
+    exact ⟨charges_topYukawa x h, charges_not_isPhenoConstrained x h, charges_yukawa x h,
+      charges_complete x h⟩
+  · intro ⟨hTop, hPheno, hY, hComplete⟩
+    /- Showing that if `x ∉ charges` and `AllowsTerm x .topYukawa`,
+      `¬ IsPhenoConstrained x`, ``¬ YukawaGeneratesDangerousAtLevel x 1`, `IsComplete x`,
+      then `False`. -/
+    by_contra hn
+    suffices hnot : ¬ ((¬ IsPhenoConstrained x ∧ ¬ YukawaGeneratesDangerousAtLevel x 1) ∧
+        AllowsTerm x topYukawa) by
+      simp_all
+    revert hn
+    rw [not_and]
+    simp only [hTop, not_true_eq_false, imp_false, Decidable.not_not]
+    suffices hmem : ∃ y ∈ charges, y ⊆ x by
+      obtain ⟨y, y_mem, hyx⟩ := hmem
+      refine subset_insert_filter_card_zero charges S5 S10 (fun x =>
+        (¬x.IsPhenoConstrained ∧ ¬x.YukawaGeneratesDangerousAtLevel 1))
+        ?_ ?_ y ?_ x hyx hsub ?_ ?_
+      · simpa using fun x y hxy h1 h2 => yukawaGeneratesDangerousAtLevel_of_subset hxy <| h1
+          fun hn => h2 <| isPhenoConstrained_mono hxy hn
+      · intro x
+        exact fun a => charges_complete x a
+      · exact y_mem
+      · intro q10
+        rw [Multiset.empty_eq_zero, Multiset.eq_zero_iff_forall_notMem]
+        simp only [Multiset.mem_filter, Multiset.mem_map, not_and, Decidable.not_not,
+          forall_exists_index, and_imp, forall_apply_eq_imp_iff₂]
+        intro z hz hzP h2
+        have h1 := charges_isPhenoClosedQ10 q10 q10.2 z hz
+        simp_all
+      · intro q5
+        rw [Multiset.empty_eq_zero, Multiset.eq_zero_iff_forall_notMem]
+        simp only [Multiset.mem_filter, Multiset.mem_map, not_and, Decidable.not_not,
+          forall_exists_index, and_imp, forall_apply_eq_imp_iff₂]
+        intro z hz hzP h2
+        have h1 := charges_isPhenoClosedQ5 q5 q5.2 z hz
+        simp_all
+    /- Getting the subset of `x` which minimally allows the top Yukawa. -/
+    obtain ⟨y, hyMem, hysubsetx⟩ : ∃ y ∈ (minimallyAllowsTermsOfFinset S5 S10 topYukawa),
+        y ⊆ x := by
+      rw [allowsTerm_iff_subset_minimallyAllowsTerm] at hTop
+      obtain ⟨y, hPower, hIrre⟩ := hTop
+      use y
+      constructor
+      · rw [← minimallyAllowsTerm_iff_mem_minimallyAllowsTermOfFinset]
+        · exact hIrre
+        · exact mem_ofFinset_antitone S5 S10 (by simpa using hPower) hsub
+      · simpa using hPower
+    obtain ⟨z, hz1, hz2⟩ := exist_completions_subset_of_complete S5 S10 y x hysubsetx hsub hComplete
+    use z
+    constructor
+    · refine charges_exist y hyMem ?_ z hz1 ?_
+      · by_contra hn
+        have := isPhenoConstrained_mono hysubsetx hn
+        simp_all
+      · apply And.intro
+        · by_contra hn
+          have := isPhenoConstrained_mono hz2 hn
+          simp_all
+        · by_contra hn
+          have := yukawaGeneratesDangerousAtLevel_of_subset hz2 hn
+          simp_all
+    · simp_all
+
+end Charges
+
+end SU5
+
+end SuperSymmetry
